new ElimFuncComp3

src/ElimFunc3.v
@@ -1,28 +1,53 @@
 Require Import Common.
-Require Import StepLib.
 
 Require Import Utopia.
 Require Import Monads.
 Require Import ListLemmas.
-Require Import Psatz.
-Require HigherValue.
+Require Import Metadata.
+Require Import HigherValue.
+Require StepLib.
 
+Definition function_name := nat.
 
-(* Uses the same syntax as ElimFunc2 *)
-Require Export ElimFunc2.
+(* List containing a flag for each argument, `true` if Elim should recurse on
+   that argument, `false` if it shouldn't.  The length gives the number of
+   arguments. *)
+Definition rec_info := list bool.
 
+Inductive expr :=
+| Value (v : value)
+| Arg
+| UpVar (idx : nat)
+| Deref (e : expr) (n : nat)
+| Call (f : expr) (a : expr)
+| MkConstr (tag : nat) (args : list expr)
+| Elim (loop : expr) (cases : list (expr * rec_info)) (target : expr)
+| MkClose (f : function_name) (free : list expr)
+.
 
-(* Continuation-based step relation *)
+Inductive is_value : expr -> Prop :=
+| IsValue : forall v, is_value (Value v).
+
+Definition env := list expr.
+
+Fixpoint unroll_elim (case : expr)
+                     (target : value)
+                     (n : nat)
+                     (rec : rec_info)
+                     (mk_rec : expr -> expr) : expr :=
+    match rec with
+    | [] => case
+    | r :: rec =>
+            let arg := Deref (Value target) n in
+            let case := Call case arg in
+            let case := if r then Call case (mk_rec arg) else case in
+            unroll_elim case target (S n) rec mk_rec
+    end.
+
 
 Inductive state :=
-| Run (e : expr) (l : list expr) (k : expr -> state)
-| Stop (e : expr).
-
-Definition state_expr s :=
-    match s with
-    | Run e _ _ => e
-    | Stop e => e
-    end.
+| Run (e : expr) (l : list value) (k : value -> state)
+| Stop (v : value).
 
 Inductive sstep (E : env) : state -> state -> Prop :=
 | SArg : forall l k v,
@@ -32,54 +57,63 @@ Inductive sstep (E : env) : state -> state -> Prop :=
         nth_error l (S n) = Some v ->
         sstep E (Run (UpVar n) l k) (k v)
 
-| SCloseStep : forall fname vs e es l k,
-        Forall value vs ->
-        ~ value e ->
-        sstep E (Run (Close fname (vs ++ [e] ++ es)) l k)
-                (Run e l (fun v => Run (Close fname (vs ++ [v] ++ es)) l k))
-| SCloseDone : forall fname vs l k,
-        Forall value vs ->
-        sstep E (Run (Close fname vs) l k) (k (Close fname vs))
+| SDerefStep : forall e n l k,
+        ~ is_value e ->
+        sstep E (Run (Deref e n) l k)
+                (Run e l (fun v => Run (Deref (Value v) n) l k))
+| SDerefinate : forall tag args n l k v,
+        nth_error args n = Some v ->
+        sstep E (Run (Deref (Value (Constr tag args)) n) l k)
+                (k v)
+
+| SCloseStep : forall tag vs e es l k,
+        Forall is_value vs ->
+        ~ is_value e ->
+        sstep E (Run (MkClose tag (vs ++ [e] ++ es)) l k)
+                (Run e l (fun v => Run (MkClose tag (vs ++ [Value v] ++ es)) l k))
+| SCloseDone : forall tag vs l k,
+        let es := map Value vs in
+        sstep E (Run (MkClose tag es) l k) (k (Close tag vs))
 
 | SConstrStep : forall fname vs e es l k,
-        Forall value vs ->
-        ~ value e ->
-        sstep E (Run (Constr fname (vs ++ [e] ++ es)) l k)
-                (Run e l (fun v => Run (Constr fname (vs ++ [v] ++ es)) l k))
+        Forall is_value vs ->
+        ~ is_value e ->
+        sstep E (Run (MkConstr fname (vs ++ [e] ++ es)) l k)
+                (Run e l (fun v => Run (MkConstr fname (vs ++ [Value v] ++ es)) l k))
 | SConstrDone : forall fname vs l k,
-        Forall value vs ->
-        sstep E (Run (Constr fname vs) l k) (k (Constr fname vs))
+        let es := map Value vs in
+        sstep E (Run (MkConstr fname es) l k) (k (Constr fname vs))
 
 | SCallL : forall e1 e2 l k,
-        ~ value e1 ->
+        ~ is_value e1 ->
         sstep E (Run (Call e1 e2) l k)
-                (Run e1 l (fun v => Run (Call v e2) l k))
+                (Run e1 l (fun v => Run (Call (Value v) e2) l k))
 | SCallR : forall e1 e2 l k,
-        value e1 ->
-        ~ value e2 ->
+        is_value e1 ->
+        ~ is_value e2 ->
         sstep E (Run (Call e1 e2) l k)
-                (Run e2 l (fun v => Run (Call e1 v) l k))
+                (Run e2 l (fun v => Run (Call e1 (Value v)) l k))
 | SMakeCall : forall fname free arg l k body,
-        Forall value free ->
-        value arg ->
         nth_error E fname = Some body ->
-        sstep E (Run (Call (Close fname free) arg) l k)
+        sstep E (Run (Call (Value (Close fname free)) (Value arg)) l k)
                 (Run body (arg :: free) k)
 
-| SElimStepRec : forall rec cases l k,
-        ~ value rec ->
-        sstep E (Run (ElimBody rec cases) l k)
-                (Run rec l (fun v => Run (ElimBody v cases) l k))
-| SEliminate : forall rec cases tag args l k case info e',
-        value rec ->
-        Forall value args ->
-        nth_error cases tag = Some (case, info) ->
-        unroll_elim rec case args info = Some e' ->
-        sstep E (Run (ElimBody rec cases) (Constr tag args :: l) k)
-                (Run e' (Constr tag args :: l) k)
+| SElimStepLoop : forall loop cases target l k,
+        ~ is_value loop ->
+        sstep E (Run (Elim loop cases target) l k)
+                (Run loop l (fun v => Run (Elim (Value v) cases target) l k))
+| SElimStep : forall loop cases target l k,
+        is_value loop ->
+        ~ is_value target ->
+        sstep E (Run (Elim loop cases target) l k)
+                (Run target l (fun v => Run (Elim loop cases (Value v)) l k))
+| SEliminate : forall loop cases tag args l k case rec e',
+        is_value loop ->
+        nth_error cases tag = Some (case, rec) ->
+        unroll_elim case (Constr tag args) 0 rec (fun x => Call loop x) = e' ->
+        sstep E (Run (Elim loop cases (Value (Constr tag args))) l k)
+                (Run e' l k)
 .
-
-
 
 Definition sstar BE := StepLib.sstar (sstep BE).
 Definition SStarNil := @StepLib.SStarNil state.
@@ -91,75 +125,144 @@ Definition SPlusCons := @StepLib.SPlusCons state.
 
 
 
-Require Import Metadata.
+
+(* Proofs *)
+
+(*
+ * Mutual recursion/induction schemes for expr
+ *)
+
+Definition expr_rect_mut
+        (P : expr -> Type)
+        (Pl : list expr -> Type)
+        (Pp : expr * rec_info -> Type)
+        (Plp : list (expr * rec_info) -> Type)
+    (HValue :   forall v, P (Value v))
+    (HArg :     P Arg)
+    (HUpVar :   forall n, P (UpVar n))
+    (HDeref :   forall e n, P e -> P (Deref e n))
+    (HCall :    forall f a, P f -> P a -> P (Call f a))
+    (HConstr :  forall tag args, Pl args -> P (MkConstr tag args))
+    (HElim :    forall loop cases target,
+        P loop -> Plp cases -> P target -> P (Elim loop cases target))
+    (HClose :   forall f free, Pl free -> P (MkClose f free))
+    (Hnil :     Pl [])
+    (Hcons :    forall e es, P e -> Pl es -> Pl (e :: es))
+    (Hpair :    forall e r, P e -> Pp (e, r))
+    (Hnil_p :   Plp [])
+    (Hcons_p :  forall p ps, Pp p -> Plp ps -> Plp (p :: ps))
+    (e : expr) : P e :=
+    let fix go e :=
+        let fix go_list es :=
+            match es as es_ return Pl es_ with
+            | [] => Hnil
+            | e :: es => Hcons e es (go e) (go_list es)
+            end in
+        let go_pair p :=
+            let '(e, r) := p in
+            Hpair e r (go e) in
+        let fix go_pair_list ps :=
+            match ps as ps_ return Plp ps_ with
+            | [] => Hnil_p
+            | p :: ps => Hcons_p p ps (go_pair p) (go_pair_list ps)
+            end in
+        match e as e_ return P e_ with
+        | Value v => HValue v
+        | Arg => HArg
+        | UpVar n => HUpVar n
+        | Deref e n => HDeref e n (go e)
+        | Call f a => HCall f a (go f) (go a)
+        | MkConstr tag args => HConstr tag args (go_list args)
+        | Elim loop cases target =>
+                HElim loop cases target (go loop) (go_pair_list cases) (go target)
+        | MkClose f free => HClose f free (go_list free)
+        end in go e.
+
+Definition expr_rect_mut'
+        (P : expr -> Type)
+        (Pl : list expr -> Type)
+        (Pp : expr * rec_info -> Type)
+        (Plp : list (expr * rec_info) -> Type)
+    HValue HArg HUpVar HDeref HCall HConstr HElim HClose Hnil Hcons Hpair Hnil_p Hcons_p
+    : (forall e, P e) * (forall es, Pl es) * (forall p, Pp p) * (forall ps, Plp ps) :=
+    let go := expr_rect_mut P Pl Pp Plp
+        HValue HArg HUpVar HDeref HCall HConstr HElim HClose Hnil Hcons Hpair Hnil_p Hcons_p
+    in
+    let fix go_list es :=
+        match es as es_ return Pl es_ with
+        | [] => Hnil
+        | e :: es => Hcons e es (go e) (go_list es)
+        end in
+    let go_pair p :=
+        let '(e, r) := p in
+        Hpair e r (go e) in
+    let fix go_pair_list ps :=
+        match ps as ps_ return Plp ps_ with
+        | [] => Hnil_p
+        | p :: ps => Hcons_p p ps (go_pair p) (go_pair_list ps)
+        end in
+    (go, go_list, go_pair, go_pair_list).
+
+(* Useful wrapper for `expr_rect_mut with (Pl := Forall P)` *)
+Definition expr_ind' (P : expr -> Prop) (Pp : (expr * rec_info) -> Prop)
+    (HValue :   forall v, P (Value v))
+    (HArg :     P Arg)
+    (HUpVar :   forall n, P (UpVar n))
+    (HDeref :   forall e n, P e -> P (Deref e n))
+    (HCall :    forall f a, P f -> P a -> P (Call f a))
+    (HConstr :  forall c args, Forall P args -> P (MkConstr c args))
+    (HElim :    forall loop cases target,
+        P loop -> Forall Pp cases -> P target -> P (Elim loop cases target))
+    (HClose :   forall f free, Forall P free -> P (MkClose f free))
+    (Hpair :    forall e r, P e -> Pp (e, r))
+    (e : expr) : P e :=
+    ltac:(refine (@expr_rect_mut P (Forall P) Pp (Forall Pp)
+        HValue HArg HUpVar HDeref HCall HConstr HElim HClose _ _ Hpair _ _ e); eauto).
+
+(* Useful wrapper for `expr_rect_mut with (Pl := Forall P)` *)
+Definition expr_ind'' (P : expr -> Prop)
+    (HValue :   forall v, P (Value v))
+    (HArg :     P Arg)
+    (HUpVar :   forall n, P (UpVar n))
+    (HDeref :   forall e n, P e -> P (Deref e n))
+    (HCall :    forall f a, P f -> P a -> P (Call f a))
+    (HConstr :  forall c args, Forall P args -> P (MkConstr c args))
+    (HElim :    forall loop cases target,
+        P loop ->
+        Forall (fun c => P (fst c)) cases ->
+        P target ->
+        P (Elim loop cases target))
+    (HClose :   forall f free, Forall P free -> P (MkClose f free))
+    (e : expr) : P e :=
+    ltac:(refine (@expr_rect_mut P (Forall P) (fun c => P (fst c)) (Forall (fun c => P (fst c)))
+        HValue HArg HUpVar HDeref HCall HConstr HElim HClose _ _ _ _ _ e); eauto).
+
+
+Require Semantics.
 
 Definition prog_type : Type := list expr * list metadata.
 Definition valtype := HigherValue.value.
 
-Inductive expr_value : expr -> valtype -> Prop :=
-| EvConstr : forall tag args1 args2,
-        Forall2 expr_value args1 args2 ->
-        expr_value (Constr tag args1)
-                   (HigherValue.Constr tag args2)
-| EvClose : forall tag free1 free2,
-        Forall2 expr_value free1 free2 ->
-        expr_value (Close tag free1)
-                   (HigherValue.Close tag free2)
-.
+Definition initial_env (prog : prog_type) : env := fst prog.
 
 Inductive is_callstate (prog : prog_type) : valtype -> valtype -> state -> Prop :=
-| IsCallstate : forall fname free free_e av ae body,
+| IsCallstate : forall fname free av body,
         nth_error (fst prog) fname = Some body ->
-        let fv := HigherValue.Close fname free in
-        expr_value ae av ->
-        Forall2 expr_value free_e free ->
+        let fv := Close fname free in
         HigherValue.public_value (snd prog) fv ->
         HigherValue.public_value (snd prog) av ->
         is_callstate prog fv av
-            (Run body (ae :: free_e) Stop).
+            (Run body (av :: free) Stop).
 
 Inductive final_state (prog : prog_type) : state -> valtype -> Prop :=
-| FinalState : forall e v,
-        expr_value e v ->
+| FinalState : forall v,
         HigherValue.public_value (snd prog) v ->
-        final_state prog (Stop e) v.
+        final_state prog (Stop v) v.
 
-Definition initial_env (prog : prog_type) : env := fst prog.
-
-Require Semantics.
 Definition semantics (prog : prog_type) : Semantics.semantics :=
   @Semantics.Semantics_gen state env valtype
                  (is_callstate prog)
                  (sstep)
-                 (* (initial_state prog) *)
                  (final_state prog)
                  (initial_env prog).
 
-
-
-Lemma expr_value_value : forall e v,
-    expr_value e v ->
-    value e.
-induction e using expr_rect_mut with
-    (Pl := fun es => forall vs,
-        Forall2 expr_value es vs ->
-        Forall value es)
-    (Pp := fun e => forall v,
-        expr_value (fst e) v ->
-        value (fst e))
-    (Plp := fun es => forall vs,
-        Forall2 (fun e v => expr_value (fst e) v) es vs ->
-        Forall (fun e => value (fst e)) es) ;
-intros0 Hev; try solve [invc Hev + simpl in *; eauto].
-
-- invc Hev. constructor. eauto.
-- invc Hev. constructor. eauto.
-Qed.
-Hint Resolve expr_value_value.
-
-Lemma expr_value_value_list : forall e v,
-    Forall2 expr_value e v ->
-    Forall value e.
-induction e; intros0 Hev; invc Hev; eauto using expr_value_value.
-Qed.
-Hint Resolve expr_value_value_list.
